Lean: refactor StrongCausalOrder monotonicity assumptions (#22)
* Refactor StrongCausalOrder monotonicity assumptions

* Include additional Lean fixes for insert and causal network

LeanYjs/Network/StrongCausalOrder.lean
@@ -83,14 +83,12 @@ class Operation (A : Type) where
   effect : A → State → Except Error State
   isValidState : A → State → Prop
   StateInv : State → Prop := fun _ => True
-  stateInv_init : StateInv init := by trivial
+  stateInv_init : StateInv init
   stateInv_effect : ∀ (op : A) (s s' : State),
     StateInv s →
     isValidState op s →
     effect op s = Except.ok s' →
-    StateInv s' := by
-      intro _ _ _ _ _ _
-      trivial
+    StateInv s'
 
 def effect_list [Operation A] (ops : List A) (s : Operation.State A) :=
   foldlM (fun s op => Operation.effect op s) s ops
@@ -110,24 +108,22 @@ def effect_list [Operation A] (ops : List A) (s : Operation.State A) :=
     simp [effect_list]
   | cons a ops₀ ih =>
     simp [effect_list]
-
-class MonotoneOperation (A : Type) {hb : CausalOrder A} (S : outParam Type) [DecidableEq S] [WithId A S] [Operation A]  [Operation A] where
-  StateSource : A → Prop := fun _ => True
-  -- TODO: is this enough to strong assumption for yjs?
-  isValidState_mono : ∀ {l : List A},
-    StateSource a →
-    (∀x < a, x ∈ l) →
-    hb_consistent hb l →
-    hbClosed hb l →
-    effect_list l Operation.init = Except.ok s →
-    IdNoDup l →
-    Operation.isValidState a s
 end effect
 
 section commutativity
 
 variable {A : Type} [DecidableEq A] {S : Type} [DecidableEq S] {hb : CausalOrder A}
 variable [WithId A S]  [Operation A]
+
+def IsValidStateMonotone (StateSource : A → Prop) : Prop :=
+  ∀ {a : A} {s : Operation.State A} {l : List A},
+    StateSource a →
+    (∀ x < a, x ∈ l) →
+    hb_consistent hb l →
+    hbClosed hb l →
+    effect_list l Operation.init = Except.ok s →
+    IdNoDup l →
+    Operation.isValidState a s
 
 def concurrent_commutative (list : List A) : Prop :=
   ∀ a b (s s' : Operation.State A), a ∈ list → b ∈ list → hb_concurrent hb a b →
@@ -147,9 +143,9 @@ theorem Except.bind_eq_ok_exist' {α β : Type} {e : Except α β} {f : β → E
     refine ⟨u, rfl, ?_⟩
     exact h
 
-theorem effect_list_stateInv [MonotoneOperation A (hb := hb) S] :
+theorem effect_list_stateInv (StateSource : A → Prop) (h_valid_mono : IsValidStateMonotone (hb := hb) StateSource) :
   ∀ {ops : List A} {s : Operation.State A},
-    (∀ op, op ∈ ops → MonotoneOperation.StateSource (A := A) (hb := hb) op) →
+    (∀ op, op ∈ ops → StateSource op) →
     hb_consistent hb ops →
     hbClosed hb ops →
     IdNoDup ops →
@@ -191,8 +187,7 @@ theorem effect_list_stateInv [MonotoneOperation A (hb := hb) S] :
           exact h_source op (by simp [hop]))
         h_consistent_ops h_closed_ops h_no_dup_ops h_prefix
     have h_valid_a : Operation.isValidState a s_prev := by
-      refine MonotoneOperation.isValidState_mono (hb := hb) (a := a) (s := s_prev)
-        (l := ops) ?_ ?_ h_consistent_ops h_closed_ops h_prefix h_no_dup_ops
+      refine h_valid_mono (a := a) (s := s_prev) (l := ops) ?_ ?_ h_consistent_ops h_closed_ops h_prefix h_no_dup_ops
       · exact h_source a (by simp)
       intro x hx_lt
       exact h_closed a x ops [] (by simp) hx_lt
@@ -295,8 +290,9 @@ theorem hb_consistent_swap (ops₀ ops₁ : List A) (a b : A) :
                 simp [List.mem_append, hy]
         exact h_no_lt_x y hy' hle
 
-theorem hb_concurrent_effect_list_reorder [MonotoneOperation A (hb := hb) S] :
-  (∀ x, x ∈ (ops₀ ++ a :: ops₁) → MonotoneOperation.StateSource (A := A) (hb := hb) x) →
+theorem hb_concurrent_effect_list_reorder (StateSource : A → Prop) (h_valid_mono : IsValidStateMonotone (hb := hb) StateSource)
+  {s : Operation.State A} :
+  (∀ x, x ∈ (ops₀ ++ a :: ops₁) → StateSource x) →
   concurrent_commutative (hb := hb) (ops₀ ++ a :: ops₁) →
   (∀ x ∈ ops₁, hb_concurrent hb x a) →
   hb_consistent hb (ops₀ ++ a :: ops₁) →
@@ -322,7 +318,7 @@ theorem hb_concurrent_effect_list_reorder [MonotoneOperation A (hb := hb) S] :
       grind [Except.bind_eq_ok_exist]
     obtain ⟨ u, h_effects_eq, h_effect_b_eq ⟩ := Except.bind_eq_ok_exist h
     have h_stateInv_u : Operation.StateInv u := by
-      apply effect_list_stateInv (hb := hb) (S := S) (ops := ops₀)
+      apply effect_list_stateInv (hb := hb) (S := S) (StateSource := StateSource) h_valid_mono (ops := ops₀)
       · intro x hx
         exact h_source x (by simp [hx])
       · apply hb_consistent_sublist (hb := hb) h_consistent
@@ -336,16 +332,14 @@ theorem hb_concurrent_effect_list_reorder [MonotoneOperation A (hb := hb) S] :
       . simp
       . grind [hb_concurrent_symm]
       . exact h_stateInv_u
-      . refine MonotoneOperation.isValidState_mono (hb := hb) (a := a) (s := u) (l := ops₀)
-          ?_ ?_ ?_ ?_ h_effects_eq ?_
+      . refine h_valid_mono (a := a) (s := u) (l := ops₀) ?_ ?_ ?_ ?_ h_effects_eq ?_
         · exact h_source a (by simp)
         · intro x hxlt
           exact h_closed a x ops₀ (b :: ops₁) (by simp [List.append_assoc]) hxlt
         · grind [hb_consistent_sublist]
         · grind [hbClosed]
         · grind [IdNoDup]
-      . refine MonotoneOperation.isValidState_mono (hb := hb) (a := b) (s := u) (l := ops₀)
-          ?_ ?_ ?_ ?_ h_effects_eq ?_
+      . refine h_valid_mono (a := b) (s := u) (l := ops₀) ?_ ?_ ?_ ?_ h_effects_eq ?_
         · exact h_source b (by simp)
         · intros x hxlt
           have h : ¬ a < b := by
@@ -494,9 +488,10 @@ theorem mem_ops0_prefix_iff_ops1
           (List.mem_append).2 (Or.inr hlast)
         simpa [List.append_assoc] using hx_all
 
-theorem hb_consistent_effect_convergent [MonotoneOperation A (hb := hb) S] (ops₀ ops₁ : List A)
-  (h_source₀ : ∀ x, x ∈ ops₀ → MonotoneOperation.StateSource (A := A) (hb := hb) x)
-  (h_source₁ : ∀ x, x ∈ ops₁ → MonotoneOperation.StateSource (A := A) (hb := hb) x)
+theorem hb_consistent_effect_convergent (StateSource : A → Prop) (h_valid_mono : IsValidStateMonotone (hb := hb) StateSource)
+  (ops₀ ops₁ : List A) (s : Operation.State A)
+  (h_source₀ : ∀ x, x ∈ ops₀ → StateSource x)
+  (h_source₁ : ∀ x, x ∈ ops₁ → StateSource x)
   (h_consistent₀ : hb_consistent hb ops₀)
   (h_consistent₁ : hb_consistent hb ops₁)
   (hclosed₀ : hbClosed hb ops₀)
@@ -583,7 +578,7 @@ by
           have ⟨ s', ⟨ h, heq ⟩  ⟩ := Except.bind_eq_ok_exist h
           simp
           have h' := h
-          apply hb_concurrent_effect_list_reorder (hb := hb) at h
+          apply hb_concurrent_effect_list_reorder (hb := hb) (StateSource := StateSource) h_valid_mono at h
           . simp at *
             rw [h', ←h]
           . intro x hx
@@ -646,7 +641,7 @@ by
           have h_closed_prefix : hbClosed hb (ops₀_first ++ ops₀_last) :=
             hbClosed_remove_concurrent (hb := hb) ops₀_first ops₀_last a b hclosed₀ h_a_concurrent_ops₀_last
           have h_stateInv_s' : Operation.StateInv s' := by
-            apply effect_list_stateInv (hb := hb) (S := S) (ops := ops₀_first ++ ops₀_last)
+            apply effect_list_stateInv (hb := hb) (S := S) (StateSource := StateSource) h_valid_mono (ops := ops₀_first ++ ops₀_last)
             · intro x hx
               exact h_source₀ x (by
                 simp [List.mem_append, List.append_assoc] at hx ⊢
@@ -679,8 +674,7 @@ by
               exact And.intro h_not_b_le_a h_not_a_le_b
             · exact h_stateInv_s'
             · -- isValidState b s'
-              refine MonotoneOperation.isValidState_mono (hb := hb) (a := b) (s := s')
-                (l := ops₀_first ++ ops₀_last) ?_ ?_ ?_ ?_ h_eff ?_
+              refine h_valid_mono (a := b) (s := s') (l := ops₀_first ++ ops₀_last) ?_ ?_ ?_ ?_ h_eff ?_
               · exact h_source₀ b (by simp [List.mem_append, List.append_assoc])
               · intro x hxlt
                 have h' := hclosed₀ b x (ops₀_first) (ops₀_last ++ [a]) (by simp [List.append_assoc]) hxlt
@@ -690,8 +684,7 @@ by
               · exact h_closed_prefix
               · grind [IdNoDup]
             · -- isValidState a s'
-              refine MonotoneOperation.isValidState_mono (hb := hb) (a := a) (s := s')
-                (l := ops₀_first ++ ops₀_last) ?_ ?_ ?_ ?_ h_eff ?_
+              refine h_valid_mono (a := a) (s := s') (l := ops₀_first ++ ops₀_last) ?_ ?_ ?_ ?_ h_eff ?_
               · exact h_source₀ a (by simp [List.mem_append, List.append_assoc])
               · intro x hxlt
                 have h' := hclosed₀ a x (ops₀_first ++ b :: ops₀_last) [] (by simp [List.append_assoc]) hxlt
